\documentclass[]{article}
\usepackage{amsmath}
%opening
\title{}
\author{}
\date{}
\begin{document}

\maketitle


\begin{gather*}
2*12^{2010} - 3 mod 13 \neq 0 \\
2*12^{2010} - 2 mod 13 =  0 \\  
Proof:\\ 
12^2  mod 13 = (144 - (130+13)) = 1 \\
Kein Taschenrechner\\
12^{2010} mod 13 = (12^2)^{1005} mod 13 \\
= 1^{1005} mod 13 = 1*1 \dots 1 mod 13 = 1 \\
\\
  2 * 12^{2010} mod 13 = 2*1 mod 13 = 2
  \\
  2 * 12^{2010} mod 13 -2  \\= 2*1 mod 13 -2 \\= 2-2  = 0\\
  2 * 12^{2010} mod 13 -3  \\= 2*1 mod 13 -3 \\= 2-3  = -1 \neq 0
  \end{gather*}


\section{}

\end{document}
